Address code review remarks

src/Init/Data/Char/Ordinal.lean
@@ -51,11 +51,11 @@ def ordinal (c : Char) : Fin Char.numCodePoints :=
   if h : c.val < 0xd800 then
     ⟨c.val.toNat, by grind [UInt32.lt_iff_toNat_lt]⟩
   else
-    ⟨c.val.toNat - Char.numSurrogates, have := c.valid; by grind [UInt32.lt_iff_toNat_lt]⟩
+    ⟨c.val.toNat - Char.numSurrogates, by grind [UInt32.lt_iff_toNat_lt]⟩
 
 /--
 Unpacks {lean}`Fin Char.numCodePoints` bijectively to {name}`Char` by shifting code points which are
-greater then the surrogate code points by the number of surrogate code points.
+greater than the surrogate code points by the number of surrogate code points.
 
 The inverse of this function is called {name}`Char.ordinal`.
 -/
@@ -79,22 +79,22 @@ def succ? (c : Char) : Option Char :=
     some ⟨0xe000, by decide⟩
   else if h₂ : c.val < 0x10ffff then
     some ⟨c.val + 1, by
-      have := c.valid
       simp only [UInt32.lt_iff_toNat_lt, UInt32.reduceToNat, Nat.not_lt, ← UInt32.toNat_inj,
         UInt32.isValidChar, Nat.isValidChar, UInt32.toNat_add, Nat.reducePow] at *
-      omega⟩
+      grind⟩
   else none
 
 /--
 Computes the {name}`m`-th next {name}`Char`, skipping over surrogate code points (which are not
 valid {name}`Char`s) as necessary.
 
-This function is specificed by its interaction with {name}`Char.ordinal`, see
+This function is specified by its interaction with {name}`Char.ordinal`, see
 {name (scope := "Init.Data.Char.Ordinal")}`Char.succMany?_eq`.
 -/
 def succMany? (m : Nat) (c : Char) : Option Char :=
   c.ordinal.addNat? m |>.map Char.ofOrdinal
 
+@[grind =]
 theorem coe_ordinal {c : Char} :
     (c.ordinal : Nat) =
       if c.val < 0xd800 then
@@ -108,6 +108,7 @@ theorem ordinal_zero : '\x00'.ordinal = 0 := by
   ext
   simp [coe_ordinal]
 
+@[grind =]
 theorem val_ofOrdinal {f : Fin Char.numCodePoints} :
     (Char.ofOrdinal f).val =
       if h : (f : Nat) < 0xd800 then
@@ -124,11 +125,8 @@ theorem ofOrdinal_ordinal {c : Char} : Char.ofOrdinal c.ordinal = c := by
   · grind [UInt32.lt_iff_toNat_lt, UInt32.ofNatLT_toNat]
   · rw [dif_neg]
     · simp only [← UInt32.toNat_inj, UInt32.toNat_add, UInt32.toNat_ofNatLT, Nat.reducePow]
-      rw [Nat.sub_add_cancel]
-      · grind [UInt32.toNat_lt]
-      · grind [UInt32.lt_iff_toNat_lt]
-    · have := c.valid
-      grind [UInt32.lt_iff_toNat_lt]
+      grind [UInt32.toNat_lt, UInt32.lt_iff_toNat_lt]
+    · grind [UInt32.lt_iff_toNat_lt]
 
 @[simp]
 theorem ordinal_ofOrdinal {f : Fin Char.numCodePoints} : (Char.ofOrdinal f).ordinal = f := by
@@ -140,7 +138,9 @@ theorem ordinal_ofOrdinal {f : Fin Char.numCodePoints} : (Char.ofOrdinal f).ordi
   · rw [if_neg, UInt32.toNat_add, UInt32.toNat_ofNatLT, UInt32.toNat_ofNatLT, Nat.mod_eq_of_lt,
       Nat.add_sub_cancel]
     · grind
-    · simpa [UInt32.lt_iff_toNat_lt] using by grind
+    · simp only [UInt32.lt_iff_toNat_lt, UInt32.toNat_add, UInt32.toNat_ofNatLT, Nat.reducePow,
+        UInt32.reduceToNat, Nat.not_lt]
+      grind
 
 @[simp]
 theorem ordinal_comp_ofOrdinal : Char.ordinal ∘ Char.ofOrdinal = id := by
@@ -166,10 +166,9 @@ theorem ofOrdinal_injective : Function.Injective Char.ofOrdinal :=
    fun _ _ => ofOrdinal_inj.1
 
 theorem ordinal_le_of_le {c d : Char} (h : c ≤ d) : c.ordinal ≤ d.ordinal := by
-  have := c.valid
-  have := d.valid
   simp only [le_def, UInt32.le_iff_toNat_le] at h
-  simpa [coe_ordinal, Fin.le_def, UInt32.lt_iff_toNat_lt] using by grind
+  simp only [Fin.le_def, coe_ordinal, UInt32.lt_iff_toNat_lt, UInt32.reduceToNat]
+  grind
 
 theorem ofOrdinal_le_of_le {f g : Fin Char.numCodePoints} (h : f ≤ g) :
     Char.ofOrdinal f ≤ Char.ofOrdinal g := by
@@ -179,7 +178,8 @@ theorem ofOrdinal_le_of_le {f g : Fin Char.numCodePoints} (h : f ≤ g) :
   · simp only [UInt32.toNat_ofNatLT]
     split
     · simpa
-    · simpa using by grind
+    · simp only [UInt32.toNat_add, UInt32.toNat_ofNatLT, Nat.reducePow]
+      grind
   · simp only [UInt32.toNat_add, UInt32.toNat_ofNatLT, Nat.reducePow]
     rw [dif_neg (by grind)]
     simp only [UInt32.toNat_add, UInt32.toNat_ofNatLT, Nat.reducePow]
@@ -206,7 +206,9 @@ theorem succ?_eq {c : Char} : c.succ? = (c.ordinal.addNat? 1).map Char.ofOrdinal
     · simp only [coe_ordinal, Option.map_some, Option.some.injEq, Char.ext_iff, val_ofOrdinal,
         UInt32.ofNatLT_add, UInt32.reduceOfNatLT]
       split
-      · simpa using by grind [UInt32.lt_iff_toNat_lt]
+      · simp only [UInt32.ofNatLT_toNat, dite_eq_ite, left_eq_ite_iff, Nat.not_lt,
+          Nat.reduceLeDiff, UInt32.left_eq_add]
+        grind [UInt32.lt_iff_toNat_lt]
       · grind
     · simp [coe_ordinal]
       grind [UInt32.lt_iff_toNat_lt]
@@ -217,18 +219,18 @@ theorem succ?_eq {c : Char} : c.succ? = (c.ordinal.addNat? 1).map Char.ofOrdinal
   | case3 =>
     rw [Fin.addNat?_eq_some]
     · simp only [coe_ordinal, Option.map_some, Option.some.injEq, Char.ext_iff, val_ofOrdinal,
-      UInt32.ofNatLT_add, UInt32.reduceOfNatLT]
+        UInt32.ofNatLT_add, UInt32.reduceOfNatLT]
       split
       · grind
       · rw [dif_neg]
-        · simpa [← UInt32.toNat_inj] using by grind [UInt32.lt_iff_toNat_lt, UInt32.toNat_inj]
-        · have := c.valid
+        · simp only [← UInt32.toNat_inj, UInt32.toNat_add, UInt32.reduceToNat, Nat.reducePow,
+            UInt32.toNat_ofNatLT, Nat.mod_add_mod]
           grind [UInt32.lt_iff_toNat_lt, UInt32.toNat_inj]
-    · simpa [coe_ordinal] using by grind [UInt32.lt_iff_toNat_lt]
+        · grind [UInt32.lt_iff_toNat_lt, UInt32.toNat_inj]
+    · grind [UInt32.lt_iff_toNat_lt]
   | case4 =>
     rw [eq_comm]
-    have := c.valid
-    simpa [coe_ordinal, Fin.addNat?_eq_none_iff] using by grind [UInt32.lt_iff_toNat_lt]
+    grind [UInt32.lt_iff_toNat_lt]
 
 theorem map_ordinal_succ? {c : Char} : c.succ?.map ordinal = c.ordinal.addNat? 1 := by
   simp [succ?_eq]
